otbn_model/spec/types.dfy
@@ -12,16 +12,16 @@ newtype{:nativeType "ulong"} ulong = i:int | 0 <= i < 0x1_0000_0000_0000_0000
 // Subset types
 /////////////////
 
-const QUARTER_BASE : int := 0x1_0000_0000_0000_0000;
-const HALF_BASE: int := 0x1_00000000_00000000_00000000_00000000;
-const BASE : int := 0x1_00000000_00000000_00000000_00000000_00000000_00000000_00000000_00000000
+const BASE_64 : int := 0x1_0000_0000_0000_0000;
+const BASE_128: int := 0x1_00000000_00000000_00000000_00000000;
+const BASE_256 : int := 0x1_00000000_00000000_00000000_00000000_00000000_00000000_00000000_00000000
 
 type uint8   = i:int | 0 <= i < 0x100
 type uint16  = i:int | 0 <= i < 0x10000
 type uint32  = i:int | 0 <= i < 0x1_0000_0000
-type uint64  = i:int | 0 <= i < QUARTER_BASE
-type uint128 = i:int | 0 <= i < HALF_BASE
-type uint256 = i:int | 0 <= i < BASE
+type uint64  = i:int | 0 <= i < BASE_64
+type uint128 = i:int | 0 <= i < BASE_128
+type uint256 = i:int | 0 <= i < BASE_256
 type Bignum = uint256
 
 /////////////////
